\section{The Convergence Rate of FTL Dynamics}\label{app:s:fictitious_convergence}
We give here the proof of the following technical lemma that we used to derive
an upper bound on the rate of convergence of the fictitious play dynamics in
Section~\ref{s:fictitious_convergence}.  We restate Lemma~\ref{l:recursion_upper_bound} for
completeness.
\repeatlemma{l:recursion_upper_bound}
% \begin{lemma}
%   Let $e(t)$ be a function satisfying the recursion
%   \[
%     e(t) =
%     \delta(t) + (1-\rho)\frac{\sum_{\tau=0}^{t-1}e(\tau)}{t}
%     \text{ and } e(0)=\|x^0 - x^*\|_{\infty},
%   \]
%   where \(\delta(t) = \sqrt{\frac{\ln(D t^2)}{t}} \), \(\delta(0) = 0 \),
%   and $D > \me^2$ is a positive constant.  Then
%   \(
%     e(t) \leq
%     \sqrt{2 \ln(D)} \frac{(\ln t)^{3/2}}{t^{\min(\rho,\, 1/2)}}.
%   \)
% \end{lemma}
\begin{proof}
  Observe that for all $t\geq 0$ the function $e(t)$ the following recursive
  relation
  \begin{equation}\label{eq:recursion}
    e(t+1) = e(t) \lp(1 - \frac{\rho}{t+1} \rp)
    + \delta(t+1)-\delta(t) + \frac{\delta(t)}{t+1}\\
  \end{equation}
  For $t=0$ we have that
  \begin{equation}\label{eq:recursion_zero}
    e(1) = (1- \rho)e(0) + \delta(1) = (1 -\rho)e(0) + \sqrt{\ln D}
  \end{equation}
  Observe that for $D>\me^2$, $\delta(t)$ is decreasing for all $t\geq 1$.
  Therefore, \(
    \delta(t+1)-\delta(t) + \frac{\delta(t)}{t+1}\leq \frac{\delta(t)}{t+1} \)
  and from equations (\ref{eq:recursion}) and (\ref{eq:recursion_zero})
  we get that for all $t\geq 0$
  \[
    e(t+1) \leq
    e(t) \lp(1 - \frac{\rho}{t+1} \rp) +
    \frac{\sqrt{\ln(D (t+1)^2)}}{(t+1)^{3/2}}
    \leq
    e(t) \lp(1 - \frac{\rho}{t+1} \rp) +
    \frac{\sqrt{2 \ln(D (t+1))}}{(t+1)^{3/2}}
  \]
  Now let \(g(t) = \frac{\sqrt{2 \ln(D t)}}{t^{3/2}} \) to obtain
  for all $t\geq 1$
  \begin{align*}
    e(t)
    &\leq
    (1-\frac{\rho}{t})e(t-1) + g(t)\\
    &\leq
    (1-\frac{\rho}{t})(1-\frac{\rho}{t-1})e(t-2)
    + (1-\frac{\rho}{t})g(t-1) + g(t)\\
    &\leq
    (1-\frac{\rho}{t})\cdots (1-\rho)e(0)
    + \sum_{\tau=1}^t g(\tau)\prod_{i=\tau+1}^t(1-\frac{\rho}{i})\\
    &\leq
    \frac{e(0)}{t^\rho}
    + \sum_{\tau=1}^tg(\tau)e^{-\rho\sum_{i=\tau+1}^t\frac{1}{i}}\\
    &\leq
    \frac{e(0)}{t^\rho}
    + \sum_{\tau=1}^tg(\tau)e^{-\rho(H_t-H_{\tau})}\\
    &\leq
    \frac{e(0)}{t^\rho}
    + e^{-\rho H_t}\sum_{\tau=1}^tg(\tau)e^{\rho H_{\tau}}\\
    &\leq
    \frac{e(0)}{t^\rho}
    + \frac{\sqrt{2}}{t^\rho}
    \sum_{\tau=1}^t\tau^\rho\frac{\sqrt{\ln (D \tau)}}{\tau^{3/2}}\\
    &\leq
    \frac{e(0)}{t^\rho}
    + \frac{\sqrt{2 \ln D }}{t^\rho}
    \sum_{\tau=1}^t\frac{\sqrt{\ln \tau}}{\tau^{3/2-\rho}}
  \end{align*}
  We observe that
  \begin{equation}\label{eq:integral_upper_bound}
    \sum_{\tau=1}^t
    \frac{\sqrt{\ln \tau}}{\tau^{3/2-\rho}}
    \leq
    \int_{\tau=1}^t \frac{\sqrt{\ln\tau}}{\tau^{3/2-\rho}}\d \tau
  \end{equation}
  since, \(\tau \mapsto \frac{\sqrt{\ln\tau}}{\tau^{3/2-\rho}}\)
  is a decreasing function of $\tau$ for all $\rho \in[0,1]$.

  \begin{itemize}
    \item If
      $\rho\leq 1/2$ then
      \[
        \int_{\tau=1}^t \tau^\rho\frac{\sqrt{\ln \tau}}{\tau^{3/2}}\d\tau
        \leq
        \sqrt{\ln t }
        \int_{\tau=1}^t
        \frac{1}{\tau}\d\tau = (\ln t)^{3/2}
      \]
    \item If $\rho > 1/2$ then\\
      \begin{align*}
        \int_{\tau=1}^t
        \tau^\rho\frac{\sqrt{\ln \tau}}{\tau^{3/2}}\d\tau
        &=
        \int_{\tau=1}^t \tau^{\rho-1/2}\frac{\sqrt{\ln \tau}}{\tau}d\tau \\
        &=
        \frac{2}{3} \int_{\tau=1}^t
        \tau^{\rho-1/2}((\ln \tau)^{3/2})'\d\tau \\
        &=
        \frac{2}{3}t^{\rho - 1/2}(\ln t)^{3/2} - (\rho-1/2)\frac{2}{3}
        \int_{\tau=1}^t \tau^{\rho-3/2}(\ln \tau)^{3/2}\d\tau \\
        &\leq \frac{2}{3} t^{\rho - 1/2}(\ln t)^{3/2}
      \end{align*}
  \end{itemize}
\end{proof}

\begin{theorem}\label{thm:convergence}
  Let $I = (P,s, \alpha)$ be any instance of the opinion formation
  game of Definition~\ref{d:random_game} with equilibrium
  $x^* \in [0,1]^n$.  The opinion vector $x(t)$ produced by
  update rule~\ref{eq:fictitious_play}
  after $t$ rounds satisfies
  \[
    \Expnew{}{\norm{\infty}{x(t) - x^*}} \leq
    C \sqrt{\log n}\frac{(\log t)^{3/2}}{t^{\min(1/2,\rho)}},
  \]
  where $\rho = \min_{i \in V} a_i$ and $C$ is a universal constant.
\end{theorem}

\begin{proof}
By Lemma~\ref{l:recursive_equation} we have that for all $t\geq 1$ and $p \in [0,1]$,
\[\Prob{\norm{\infty}{x(t)-x^*} \leq e_p(t)} \geq 1-p\]
where $e_p(t)$ is the solution of the recursion, $e_p(t) =\delta(t) + (1-\rho)\frac{\sum_{\tau=0}^{t-1}e_p(\tau)}{t}$ with
$\delta(t)=\sqrt{ \frac{\log(\pi^2 n t^2/(6 p))}{t}}$. Setting $p=\frac{1}{12\sqrt{t}}$ we have that
\[\Prob{\norm{\infty}{x(t)-x^*} \leq e(t)} \geq 1-\frac{1}{12\sqrt{t}}\]
where $e(t)$ is the solution of the recursion $e(t) =\delta(t) + (1-\rho)\frac{\sum_{\tau=0}^{t-1}e_p(\tau)}{t}$ with
$\delta(t)=\sqrt{\frac{\log(2\pi^2 n t^{2.5})}{t}}$. Since $2\pi^2 \geq e^{2.5}$, Lemma~\ref{l:recursion_upper_bound} applies and
$e(t)\leq C\sqrt{\log n}\frac{\log t^{3/2}}{t^{\min(\rho,1/2)}}$ for some universal constant $C$. Finally,
\[\Expnew{}{\norm{\infty}{x(t) - x^*}} \leq \frac{1}{12\sqrt{t}} + (1-\frac{1}{12\sqrt{t}})C\sqrt{\log n}\frac{(\log t)^{3/2}}{t^{\min(\rho,1/2)}}
\leq (C+\frac{1}{12})\sqrt{\log n}\frac{(\log t)^{3/2}}{t^{\min(\rho,1/2)}}\]
\end{proof}
