\section{FTL dynamics has no-regret}\label{app:s:fictitious_noregret}
We prove here Lemma~\ref{l:y_t}, which we restate for
convenience.
\begin{lemma}
Let $\{b_t\}_{t=0}^\infty$ be an arbitrary sequence with $b_t \in [0,1]$. Let $y_t = \argmin_{x \in [0,1]}\sum_{\tau=0}^tf(x_,b_\tau)$
then for all $t$,
\[
\sum_{\tau=0}^t f(y_\tau,b_\tau) \leq \min_{x \in [0,1]}\sum_{\tau = 0}^tf(x,b_\tau)
\]
\end{lemma}
\begin{proof}By definition of $y_t$,
  $\sum_{\tau=0}^t f(y_t,b_\tau)=\min_{ x \in [0,1]} \sum_{\tau=0}^t f(x,b_\tau)$, so
  \begin{align*}
    \sum_{\tau=0}^t f(y_\tau,b_\tau) - \min_{ x \in [0,1]} \sum_{\tau=0}^t f(x,b_\tau) &=
    \sum_{\tau=0}^t f(y_\tau,b_\tau) - \sum_{\tau=0}^t f(y_t,b_\tau)\\
    &= \sum_{\tau=0}^{t-1} f(y_\tau,b_\tau) - \sum_{\tau=0}^{t-1} f(y_t,b_\tau)\\
    &\leq \sum_{\tau=0}^{t-1} f(y_\tau,b_\tau) - \sum_{\tau=0}^{t-1} f(y_{t-1},b_\tau)\\
%    &= \sum_{\tau=0}^{t-2} f(y_\tau,b_\tau) - \sum_{\tau=0}^{t-2}f(y_{t-1},b_\tau)
  \end{align*}
  The last inequality follows by the fact that $y_{t-1} = \argmin_{x \in [0,1]}\sum_{\tau=0}^{t-1}f(x_,b_\tau)$
  Inductively, we prove that $\sum_{\tau=0}^t f(y_\tau,b_\tau) \leq \min_{ x \in [0,1]} \sum_{\tau=0}^t f(x,b_\tau)$.
\end{proof}

We next prove Lemma~\ref{l:no_regret_lemma} which we combine with
Lemma~\ref{l:y_t} to show that the update rule~\ref{eq:fictitious_play}
ensures no regret for the agents. We first restate the Lemma for
convenience.
\begin{lemma}
  For all $t\geq 0$,
  \(
    f(x_t,b_t) \leq f(y_t,b_t) + 2\frac{1-\alpha}{t+1} +
    \frac{(1-\alpha)^2}{(t+1)^2}
  \).
\end{lemma}
\begin{proof}
  We first prove that for all $t$,
  \begin{equation}\label{eq:abs_value}
    \lp|x_t - y_t \rp| \leq \frac{1-\alpha}{t+1}.
  \end{equation}
  By definition
  \(x_t = \alpha s + (1-\alpha)\frac{\sum_{\tau = 0}^{t-1} b_\tau}{t}\)
  and
  \( y_t = \alpha s + (1-\alpha)\frac{\sum_{\tau = 0}^t b_\tau}{t+1}\).
  \begin{align*}
    \lp|x_t - y_t\rp|
    &=
    (1-\alpha)\lp|\frac{\sum_{\tau = 0}^{t-1}b_\tau}{t}
    - \frac{\sum_{\tau = 0}^t b_\tau}{t+1}\rp|\\
    &=
    (1-\alpha)\lp|\frac{\sum_{\tau = 0}^{t-1}b_\tau -tb_t}{t(t+1)}\rp|\\
    &\leq
    \frac{1-\alpha}{t+1}
  \end{align*}
  The last inequality follows from the fact that $b_\tau \in [0,1]$.
  We now use inequality~(\ref{eq:abs_value}) to bound the difference
  \( f(x_t,b_t) - f(y_t,b_t) \).
  \begin{align*}
    f(x_t,b_t)
    &=
    \alpha(x_t - s)^2 + (1 - \alpha)(x_t - y_t)^2 \\
    &\leq
    \alpha(y_t - s)^2 + 2\alpha\lp|y_t -
    s\rp|\lp|x_t - y_t\rp| + \alpha \lp|x_t - y_t\rp|^2 \\
    &\quad + (1-\alpha)(y_t - y_t)^2 +
    2(1-\alpha)\lp|y_t - y_t\rp|\lp|x_t-y_t\rp| + (1 - \alpha)\lp|x_t - y_t\rp|^2\\
    &\leq
    f(y_t,b_t) + 2\lp|x_t - y_t\rp| + \lp|y_t - x_t\rp|^2\\
    &\leq
    f(y_t,b_t) + 2\frac{1-\alpha}{t+1} + \frac{(1-\alpha)^2}{(t+1)^2}
  \end{align*}
\end{proof}
